feat: implement ceval (minus conditional guard failure)

P1-PL/RelationalEvaluation.v
@@ -34,6 +34,55 @@ Inductive ceval : com -> state -> list (state * com) ->
           result -> state -> list (state * com) -> Prop :=
 | E_Skip : forall st q,
  st / q =[ skip ]=> st / q / Success
+| E_Asgn : forall st q X a,
+ st / q =[ X := a ]=> (X !-> aeval st a ; st) / q / Success
+| E_Seq : forall st1 q1 c1 st2 q2 c2 st3 q3 r,
+  st1 / q1 =[ c1 ]=> st2 / q2 / Success ->
+  st2 / q2 =[ c2 ]=> st3 / q3 / r ->
+  st1 / q1 =[ c1 ; c2 ]=> st3 / q3 / r (* Do we need to check for FAIL? *)
+| E_IfTrue : forall st q b c1 c2,
+  beval st b = true ->
+  st / q =[ c1 ]=> st / q / Success -> (* Do we need to check for FAIL? *)
+  st / q =[ if b then c1 else c2 end ]=> st / q / Success
+| E_IfFalse : forall st q b c1 c2,
+  beval st b = false ->
+  st / q =[ c2 ]=> st / q / Success -> (* Do we need to check for FAIL? *)
+  st / q =[ if b then c1 else c2 end ]=> st / q / Success
+| E_WhileFalse : forall b st q c,
+  beval st b = false ->
+  st / q =[ while b do c end ]=> st / q / Success
+| E_WhileTrue : forall b st1 q1 c st2 q2 st3 q3 r,
+  beval st1 b = true -> (* If true *)
+  st1 / q1 =[ c ]=> st2 / q2 / Success -> (* Execute c *)
+  st2 / q2 =[ while b do c end ]=> st3 / q3 / r -> (* Start next iteration with new state *)
+  st1 / q1 =[ while b do c end ]=> st3 / q3 / r
+| E_NonDet1 : forall st q c1 c2,
+  st / q =[ c1 !! c2 ]=> st / ((st, c2) :: q) / Success
+| E_NonDet2 : forall st q c1 c2, (* Are both cases needed? *)
+  st / q =[ c1 !! c2 ]=> st / ((st, c1) :: q) / Success
+| E_GuardTrue : forall st q b c,
+  beval st b = true -> (* if the guard condition is true *)
+  st / q =[ (b -> c) ]=> st / q / Success
+| E_GuardFalse_NoCont : forall st q b c,
+  beval st b = false -> (* if the guard condition is false *)
+  q = [] -> (* No remaining non-deterministic choices to execute *)
+  st / q =[ (b -> c) ]=> st / q / Fail
+(* | E_GuardFalse_Cont : forall st q b c st' q',
+  beval st b = false -> (* if the guard condition is false *)
+  q = (st', c) :: q' -> (* Backtrack non-deterministic choice *)
+  st' / q' =[ (b -> c) ]=> st / q / Success 
+  
+  This case is still wrong, I think.
+  
+  We ought to:
+    - start at state st / q
+    - See that beval st b = false
+    - backtrack to state st' / q' and execute command c
+        - q' is q without the state we are now backtracking to 
+    - Get to a new state st'' / q''
+  *)
+
+
 (* TODO. Hint: follow the same structure as shown in the chapter Imp *)
 where "st1 '/' q1 '=[' c ']=>' st2 '/' q2 '/' r" := (ceval c st1 q1 r st2 q2).
 
